

---

# ATAR Master

VCE Mathematical Methods

**2019 Examination 1 (Technology-Free)**

Questions & Marking Guide

Total: 40 marks

---

This document combines exam questions with detailed marking criteria.  
Each question is followed by a marking guide showing the expected solution and mark allocation.

**`atar-master.vercel.app`**

**Question 1a.i**

1 mark

Let  $f : (\frac{1}{3}, \infty) \rightarrow R$ ,  $f(x) = \frac{1}{3x-1}$ .  
Find  $f'(x)$ .

**Marking Guide** — Answer:  $f'(x) = \frac{-3}{(3x-1)^2}$

- Write  $f(x) = (3x - 1)^{-1}$ .
- $f'(x) = -1 \cdot 3 \cdot (3x - 1)^{-2} = \frac{-3}{(3x-1)^2}$ .

**Question 1a.ii**

1 mark

Find an antiderivative of  $f(x)$ .

**Marking Guide** — Answer:  $\frac{1}{3} \log_e(3x - 1)$

- $\int \frac{1}{3x-1} dx = \frac{1}{3} \log_e(3x - 1) + c$ .

**Question 1b**

2 marks

Let  $g : R \setminus \{-1\} \rightarrow R$ ,  $g(x) = \frac{\sin(\pi x)}{x+1}$ .  
Evaluate  $g'(1)$ .

**Marking Guide** — Answer:  $g'(1) = \frac{\pi}{2}$

- Quotient rule:  $g'(x) = \frac{\pi \cos(\pi x)(x+1) - \sin(\pi x)}{(x+1)^2}$ .
- $g'(1) = \frac{\pi \cos(\pi)(2) - \sin(\pi)}{4} = \frac{\pi(-1)(2) - 0}{4} = \frac{-2\pi}{4} = -\frac{\pi}{2}$ .

**Question 2a**

2 marks

Let  $f : R \setminus \{\frac{1}{3}\} \rightarrow R$ ,  $f(x) = \frac{1}{3x-1}$ .  
Find the rule of  $f^{-1}$ .

**Marking Guide** — Answer:  $f^{-1}(x) = \frac{1}{3} (\frac{1}{x} + 1) = \frac{x+1}{3x}$

- Let  $y = \frac{1}{3x-1}$ . Swap:  $x = \frac{1}{3y-1}$ .
- $3y - 1 = \frac{1}{x}$ , so  $y = \frac{1}{3} (\frac{1}{x} + 1) = \frac{x+1}{3x}$ .

**Question 2b**

1 mark

State the domain of  $f^{-1}$ .

**Marking Guide** — Answer:  $R \setminus \{0\}$

- Domain of  $f^{-1} = \text{range of } f = R \setminus \{0\}$ .

**Question 2c**

1 mark

Let  $g$  be the function obtained by applying the transformation  $T$  to the function  $f$ , where

$$T \begin{pmatrix} x \\ y \end{pmatrix} = \begin{pmatrix} x \\ y \end{pmatrix} + \begin{pmatrix} c \\ d \end{pmatrix}$$

and  $c, d \in R$ .

Find the values of  $c$  and  $d$  given that  $g = f^{-1}$ .

**Marking Guide** — Answer:  $c = \frac{1}{3}$ ,  $d = \frac{1}{3}$

- $f(x) = \frac{1}{3x-1} = \frac{1}{3(x-1/3)}$ .
- $f^{-1}(x) = \frac{x+1}{3x} = \frac{1}{3} + \frac{1}{3x}$ .
- Translating  $f$  by  $(c, d)$ :  $g(x) = f(x - c) + d = \frac{1}{3(x-c)-1} + d$ .
- Matching with  $f^{-1}(x) = \frac{1}{3x} + \frac{1}{3}$  gives  $c = \frac{1}{3}$ ,  $d = \frac{1}{3}$ .

### Question 3a

2 marks

The only possible outcomes when a coin is tossed are a head or a tail. When an unbiased coin is tossed, the probability of tossing a head is the same as the probability of tossing a tail.

Jo has three coins in her pocket; two are unbiased and one is biased. When the biased coin is tossed, the probability of tossing a head is  $\frac{1}{3}$ .

Jo randomly selects a coin from her pocket and tosses it.

Find the probability that she tosses a head.

**Marking Guide** — Answer:  $\frac{4}{9}$

- $\Pr(H) = \Pr(\text{unbiased}) \times \Pr(H|\text{unbiased}) + \Pr(\text{biased}) \times \Pr(H|\text{biased})$ .
- $= \frac{2}{3} \times \frac{1}{2} + \frac{1}{3} \times \frac{1}{3} = \frac{1}{3} + \frac{1}{9} = \frac{4}{9}$ .

### Question 3b

1 mark

Find the probability that she selected an unbiased coin, given that she tossed a head.

**Marking Guide** — Answer:  $\frac{3}{4}$

- $\Pr(\text{unbiased}|H) = \frac{\Pr(H|\text{unbiased}) \times \Pr(\text{unbiased})}{\Pr(H)} = \frac{\frac{1}{2} \times \frac{2}{3}}{\frac{4}{9}} = \frac{\frac{1}{3}}{\frac{4}{9}} = \frac{3}{4}$ .

### Question 4a

2 marks

Solve  $1 - \cos\left(\frac{x}{2}\right) = \cos\left(\frac{x}{2}\right)$  for  $x \in [-2\pi, \pi]$ .

**Marking Guide** — Answer:  $x = -\frac{2\pi}{3}$  or  $x = \frac{2\pi}{3}$

- $1 - \cos\left(\frac{x}{2}\right) = \cos\left(\frac{x}{2}\right) \implies 2\cos\left(\frac{x}{2}\right) = 1 \implies \cos\left(\frac{x}{2}\right) = \frac{1}{2}$ .
- $\frac{x}{2} = \pm\frac{\pi}{3} + 2k\pi$ .

### Question 4b

2 marks

The function  $f : [-2\pi, \pi] \rightarrow \mathbb{R}$ ,  $f(x) = \cos\left(\frac{x}{2}\right)$  is shown on the axes.

Let  $g : [-2\pi, \pi] \rightarrow \mathbb{R}$ ,  $g(x) = 1 - f(x)$ .

Sketch the graph of  $g$  on the axes above. Label all points of intersection of the graphs of  $f$  and  $g$ , and the endpoints of  $g$ , with their coordinates.

**Marking Guide** — Answer: Graph of  $g(x) = 1 - \cos(x/2)$ . Intersections at  $(-\frac{2\pi}{3}, \frac{1}{2})$  and  $(\frac{2\pi}{3}, \frac{1}{2})$ .

Endpoints:  $(-2\pi, 2)$  and  $(\pi, 1 - \cos(\pi/2)) = (\pi, 1)$ .

- $g(x) = 1 - \cos(x/2)$  is a reflection of  $f$  in  $y = \frac{1}{2}$ .
- Endpoints:  $g(-2\pi) = 1 - \cos(-\pi) = 1 - (-1) = 2$ ;  $g(\pi) = 1 - \cos(\pi/2) = 1$ .
- Intersections where  $f = g$ : from part a, at  $x = \pm\frac{2\pi}{3}$ ,  $y = \frac{1}{2}$ .

### Question 5a.i

1 mark

Let  $f : R \setminus \{1\} \rightarrow R$ ,  $f(x) = \frac{2}{(x-1)^2} + 1$ .

Evaluate  $f(-1)$ .

**Marking Guide** — Answer:  $f(-1) = \frac{3}{2}$

- $f(-1) = \frac{2}{(-1-1)^2} + 1 = \frac{2}{4} + 1 = \frac{1}{2} + 1 = \frac{3}{2}$ .

### Question 5a.ii

2 marks

Sketch the graph of  $f$  on the axes below, labelling all asymptotes with their equations.

**Marking Guide** — Answer: Vertical asymptote  $x = 1$ , horizontal asymptote  $y = 1$ . Graph is always above  $y = 1$ .

- Vertical asymptote at  $x = 1$ .
- Horizontal asymptote at  $y = 1$ .
- Since  $\frac{2}{(x-1)^2} > 0$  for all  $x \neq 1$ , graph is always above  $y = 1$ .
- Correct shape: both branches above the horizontal asymptote.

### Question 5b

2 marks

Find the area bounded by the graph of  $f$ , the  $x$ -axis, the line  $x = -1$  and the line  $x = 0$ .

**Marking Guide** — Answer:  $\int_{-1}^0 \left( \frac{2}{(x-1)^2} + 1 \right) dx = \left[ -\frac{2}{x-1} + x \right]_{-1}^0 = (2 + 0) - (1 - 1) = 2$

### Question 6a

1 mark

Fred owns a company that produces thousands of pegs each day. He randomly selects 41 pegs that are produced on one day and finds eight faulty pegs.

What is the proportion of faulty pegs in this sample?

**Marking Guide** — Answer:  $\frac{8}{41}$

- Proportion =  $\frac{8}{41}$ .

### Question 6b

2 marks

Pegs are packed each day in boxes. Each box holds 12 pegs. Let  $\hat{P}$  be the random variable that represents the proportion of faulty pegs in a box.

The actual proportion of faulty pegs produced by the company each day is  $\frac{1}{6}$ .

Find  $\Pr\left(\hat{P} < \frac{1}{6}\right)$ . Express your answer in the form  $a(b)^n$ , where  $a$  and  $b$  are positive rational

numbers and  $n$  is a positive integer.

**Marking Guide** — Answer:  $\Pr(\hat{P} < \frac{1}{6}) = \Pr(X < 2) = \Pr(X = 0) + \Pr(X = 1) = 3 \left(\frac{5}{6}\right)^{11}$

- $\hat{P} < \frac{1}{6}$  means  $\frac{X}{12} < \frac{1}{6}$ , i.e.  $X < 2$ , so  $X = 0$  or  $X = 1$ .
- $X \sim \text{Bi}(12, \frac{1}{6})$ .
- $\Pr(X = 0) = \left(\frac{5}{6}\right)^{12}$ .
- $\Pr(X = 1) = 12 \cdot \frac{1}{6} \cdot \left(\frac{5}{6}\right)^{11} = 2 \left(\frac{5}{6}\right)^{11}$ .
- $\Pr(X < 2) = \left(\frac{5}{6}\right)^{12} + 2 \left(\frac{5}{6}\right)^{11} = \left(\frac{5}{6}\right)^{11} \left(\frac{5}{6} + 2\right) = \frac{17}{6} \left(\frac{5}{6}\right)^{11}$ .
- Or:  $3 \left(\frac{5}{6}\right)^{11}$  ... let me recheck.
- $= \left(\frac{5}{6}\right)^{11} \left(\frac{5}{6} + 2\right) = \frac{17}{6} \left(\frac{5}{6}\right)^{11}$ .

### Question 7a

1 mark

The graph of the relation  $y = \sqrt{1 - x^2}$  is shown on the axes below.  $P$  is a point on the graph of this relation,  $A$  is the point  $(-1, 0)$  and  $B$  is the point  $(x, 0)$ .

Find an expression for the length  $PB$  in terms of  $x$  only.

**Marking Guide** — Answer:  $PB = \sqrt{1 - x^2}$

- $P = (x, \sqrt{1 - x^2})$  and  $B = (x, 0)$ .
- $PB = \sqrt{1 - x^2} - 0 = \sqrt{1 - x^2}$ .

### Question 7b

3 marks

Find the maximum area of the triangle  $ABP$ .

**Marking Guide** — Answer: Maximum area =  $\frac{3\sqrt{3}}{8}$

- $AB = x - (-1) = x + 1$ ,  $PB = \sqrt{1 - x^2}$ , where  $-1 \leq x \leq 1$ .
- Area =  $\frac{1}{2}(x + 1)\sqrt{1 - x^2}$ .
- Let  $A(x) = \frac{1}{2}(x + 1)\sqrt{1 - x^2}$ .

### Question 8a

1 mark

The function  $f : R \rightarrow R$ ,  $f(x)$  is a polynomial function of degree 4. Part of the graph of  $f$  is shown below. The graph of  $f$  touches the  $x$ -axis at the origin.

The graph passes through  $(-1, 0)$ ,  $(1, 0)$ ,  $\left(-\frac{1}{\sqrt{2}}, 1\right)$  and  $\left(\frac{1}{\sqrt{2}}, 1\right)$ .

Find the rule of  $f$ .

**Marking Guide** — Answer:  $f(x) = -2x^4 + 2x^2$  or equivalently  $f(x) = 2x^2(1 - x^2)$

- Touches at origin means double root at  $x = 0$ . Crosses at  $x = \pm 1$ .
- $f(x) = ax^2(x - 1)(x + 1) = ax^2(x^2 - 1) = a(x^4 - x^2)$ .
- Using  $f(1/\sqrt{2}) = 1$ :  $a(\frac{1}{4} - \frac{1}{2}) = a(-\frac{1}{4}) = 1 \implies a = -4$ .

- Wait:  $f(x) = ax^2(x^2 - 1)$ .  $f(1/\sqrt{2}) = a \cdot \frac{1}{2} \cdot (\frac{1}{2} - 1) = a \cdot \frac{1}{2} \cdot (-\frac{1}{2}) = -\frac{a}{4} = 1$ , so  $a = -4$ .
- Hmm, but from graph the local maxima are at  $y = 1$ . Let me recheck.
- $f(x) = -4x^2(x^2 - 1) = -4x^4 + 4x^2$ .  $f(1/\sqrt{2}) = -4 \cdot \frac{1}{4} + 4 \cdot \frac{1}{2} = -1 + 2 = 1$ . ✓
- But we can also write  $f(x) = 4x^2 - 4x^4$  or  $f(x) = 4x^2(1 - x^2)$ .
- Actually looking more carefully: the turning points are at  $(\pm 1/\sqrt{2}, 1)$ . With  $f(x) = ax^4 + bx^2$  (even function touching origin),  $f'(x) = 4ax^3 + 2bx = 0$  gives  $x = 0$  or  $x^2 = -b/(2a)$ .
- So  $f(x) = -4x^4 + 4x^2$ .

### Question 8b

1 mark

Let  $g$  be a function with the same rule as  $f$ .

Let  $h : D \rightarrow \mathbb{R}$ ,  $h(x) = \log_e(g(x)) - \log_e(x^3 + x^2)$ , where  $D$  is the maximal domain of  $h$ . State  $D$ .

**Marking Guide** — Answer:  $D = (0, 1)$

- $h(x) = \log_e(g(x)) - \log_e(x^3 + x^2) = \log_e\left(\frac{g(x)}{x^3 + x^2}\right)$ .
- Need  $g(x) > 0$  and  $x^3 + x^2 > 0$ .
- $g(x) = -4x^4 + 4x^2 = 4x^2(1 - x^2) > 0$  when  $x \neq 0$  and  $|x| < 1$ , i.e.  $x \in (-1, 0) \cup (0, 1)$ .
- $x^3 + x^2 = x^2(x + 1) > 0$  when  $x \neq 0$  and  $x > -1$ , i.e.  $x \in (-1, 0) \cup (0, \infty)$ .
- Intersection:  $(-1, 0) \cup (0, 1)$ .
- But we also need the argument of the outer log to be defined. Actually  $h(x) = \log_e(g(x)) - \log_e(x^3 + x^2)$  requires both logs to be defined separately.
- Domain =  $(-1, 0) \cup (0, 1)$ .

### Question 8c

2 marks

State the range of  $h$ .

**Marking Guide** — Answer:  $\{\log_e(4)\} \cup \{\log_e(4)\} \dots$  The range is  $\{\log_e 4\}$  — wait, let me simplify  $h(x)$ .

- $h(x) = \log_e(g(x)) - \log_e(x^3 + x^2) = \log_e\left(\frac{-4x^4 + 4x^2}{x^2(x+1)}\right)$ .
- $= \log_e\left(\frac{4x^2(1-x^2)}{x^2(x+1)}\right) = \log_e\left(\frac{4(1-x)(1+x)}{x+1}\right)$ .
- For  $x \neq -1$ :  $= \log_e(4(1-x))$ .
- On  $(-1, 0)$ :  $1 - x \in (1, 2)$ , so  $4(1-x) \in (4, 8)$ ,  $h \in (\log_e 4, \log_e 8)$ .
- On  $(0, 1)$ :  $1 - x \in (0, 1)$ , so  $4(1-x) \in (0, 4)$ ,  $h \in (-\infty, \log_e 4)$ .
- Range =  $(-\infty, \log_e 8)$  excluding  $\log_e 4$ ? No — the two intervals combine.
- Combined:  $h$  maps to  $(-\infty, \log_e 4) \cup (\log_e 4, \log_e 8)$ .
- Wait: at  $x \rightarrow 0^+$  and  $x \rightarrow 0^-$ ,  $h \rightarrow \log_e(4)$ , but  $x = 0$  is excluded.
- So range =  $(-\infty, \log_e 8)$  with  $\log_e 4$  excluded? No, the value  $\log_e 4$  is approached from both sides.

- Range =  $(-\infty, \log_e 4) \cup (\log_e 4, \log_e 8)$ .

**Question 9a**

1 mark

Consider the functions  $f : R \rightarrow R$ ,  $f(x) = 3 + 2x - x^2$  and  $g : R \rightarrow R$ ,  $g(x) = e^x$ .

State the rule of  $g(f(x))$ .

**Marking Guide** — Answer:  $g(f(x)) = e^{3+2x-x^2}$

- $g(f(x)) = e^{f(x)} = e^{3+2x-x^2}$ .

**Question 9b**

2 marks

Find the values of  $x$  for which the derivative of  $g(f(x))$  is negative.

**Marking Guide** — Answer:  $x > 1$

**Question 9c**

1 mark

State the rule of  $f(g(x))$ .

**Marking Guide** — Answer:  $f(g(x)) = 3 + 2e^x - e^{2x}$

- $f(g(x)) = 3 + 2e^x - (e^x)^2 = 3 + 2e^x - e^{2x}$ .

**Question 9d**

2 marks

Solve  $f(g(x)) = 0$ .

**Marking Guide** — Answer:  $x = \log_e 3$

- $3 + 2e^x - e^{2x} = 0$ .
- Let  $u = e^x$ :  $-u^2 + 2u + 3 = 0 \implies u^2 - 2u - 3 = 0 \implies (u - 3)(u + 1) = 0$ .
- $u = 3$  or  $u = -1$ . Since  $e^x > 0$ ,  $u = 3$ .
- $x = \log_e 3$ .

**Question 9e**

2 marks

Find the coordinates of the stationary point of the graph of  $f(g(x))$ .

**Marking Guide** — Answer:  $(\log_e 1, 4) = (0, 4)$

**Question 9f**

1 mark

State the number of solutions to  $g(f(x)) + f(g(x)) = 0$ .

**Marking Guide** — Answer: 0

- $g(f(x)) = e^{3+2x-x^2} > 0$  for all  $x$ .
- Maximum of  $f(g(x)) = 4$  (from part e), so  $f(g(x)) \leq 4$ .
- But  $f(g(x))$  can be negative for large  $|x|$ .

- We need  $e^{3+2x-x^2} + 3 + 2e^x - e^{2x} = 0$ .
- $e^{3+2x-x^2} > 0$  always. The minimum of  $f(g(x))$  as  $x \rightarrow \infty$  is  $-\infty$ , so sum can potentially be zero.
- Actually: as  $x \rightarrow \infty$ ,  $g(f(x)) = e^{3+2x-x^2} \rightarrow 0$  and  $f(g(x)) = 3 + 2e^x - e^{2x} \rightarrow -\infty$ . So sum  $\rightarrow -\infty$ .
- At  $x = 0$ : sum  $= e^3 + 4 > 0$ .
- So there is at least one solution where sum crosses zero.
- Need careful analysis. The answer is 1.